\documentclass[a4paper, 12pt]{scrartcl}

\usepackage[utf8]{inputenc}
\usepackage[T1]{fontenc}
\usepackage[ngerman]{babel}

\usepackage{amsmath}
\usepackage{amssymb}

\begin{document}

\[
    \sum_{i=1}^{n}(x_i-\bar{x})(y_i-\bar{y})
\]
%
\[
    \left[
    \sum_{i=1}^{n}(x_i-\bar{x})^{2} \sum_{i=1}^{n}(y_i-\bar{y})^{2}
    \right]^{1/2}
\]
%
\[
    R=\frac{\sum_{i=1}^{n}(x_i-\bar{x})(y_i-\bar{y})}{\left[
    \sum_{i=1}^{n}(x_i-\bar{x})^{2} \sum_{i=1}^{n}(y_i-\bar{y})^{2}
    \right]^{1/2}}
\]
%
\begin{gather*}
    \sum_{i=1}^{n}(x_i-\bar{x})(y_i-\bar{y})
    \\[1cm]
    \left[
    \sum_{i=1}^{n}(x_i-\bar{x})^{2} \sum_{i=1}^{n}(y_i-\bar{y})^{2}
    \right]^{1/2}
    \\[1cm]
    R=\frac{\sum_{i=1}^{n}(x_i-\bar{x})(y_i-\bar{y})}{\left[
    \sum_{i=1}^{n}(x_i-\bar{x})^{2} \sum_{i=1}^{n}(y_i-\bar{y})^{2}
    \right]^{1/2}}
\end{gather*}
%
\begin{large}
    Satz des Pythagoras:
    \begin{equation*}
        c = \sqrt{a^{2}+b^{2}}
    \end{equation*}
\end{large}
%
%
Seien $\mathbf{a,b \in\mathbb{R}, \textrm{dann gilt } (a+b)^{2}=a^{2}+2ab+b^{2}}$
\end{document}